examples/cells: Add an example using stack allocation

src/Rupicola/Examples/Cells/IndirectAdd.v
@@ -57,6 +57,9 @@ Section with_parameters.
 
       (let v := v in
        forall m,
+         (* FIXME would like to prove this:
+            (forall Ra, sep (cell_value pa a) Ra m ->
+                        sep (cell_value pa v) Ra m) -> *)
          sep (cell_value pa v) Ra m ->
          (<{ Trace := tr;
              Memory := m;
@@ -144,12 +147,193 @@ Section with_parameters.
       ensures t' m' :=
         t = t' /\ m' =* cell_value pout (indirect_add_three' a b c) * R }.
 
-  (* TODO: plug in alloc derivation
+  (* FIXME replace original compile_alloc with this. *)
+  Lemma compile_alloc
+        {tr m l functions A} (v : A):
+    forall {P} {pred: P v -> predicate} {k: nlet_eq_k P v} {k_impl}
+           {I} {AP : I -> word.rep -> A -> map.rep -> Prop} `{@Allocable _ _ _ I A AP}
+           out_var,
+
+      (forall i out_ptr uninit m',
+          (* There may be more than one predicate about m, and we're not sure
+             yet which one to use; see FAQ. *)
+         (forall (R: mem -> Prop), R m -> sep (AP i out_ptr uninit) R m') ->
+         (<{ Trace := tr;
+             Memory := m';
+             Locals := map.put l out_var out_ptr;
+             Functions := functions }>
+          k_impl
+          <{ pred_sep (Memory.anybytes out_ptr size_in_bytes) pred (nlet_eq [out_var] v k) }>)) ->
+      <{ Trace := tr;
+         Memory := m;
+         Locals := l;
+         Functions := functions }>
+      cmd.stackalloc out_var size_in_bytes k_impl
+      <{ pred (nlet_eq [out_var] (alloc v) k) }>.
+  Proof.
+    repeat straightline.
+    split; eauto using size_in_bytes_mod.
+    intros out_ptr mStack mCombined Hplace%P_from_bytes.
+    destruct Hplace as [i [out Hout]].
+    repeat straightline.
+    specialize (H0 i out_ptr out mCombined).
+    eapply WeakestPrecondition_weaken
+      with (p1 := pred_sep (Memory.anybytes out_ptr size_in_bytes)
+                           pred (let/n x as out_var eq:Heq := v in
+                                 k x Heq)).
+    2:{
+      eapply H0.
+      exists mStack; exists m;
+        intuition.
+      apply map.split_comm; eauto.
+    }
+    {
+      clear H0.
+      unfold pred_sep;
+        unfold Basics.flip;
+        simpl.
+      intros.
+      destruct H0 as [mem1 [mem2 ?]].
+      exists mem2; exists mem1;
+        intuition.
+      apply map.split_comm; eauto.
+    }
+  Qed.
+
+  Ltac cleanup_alloc :=
+    intros;
+    repeat match goal with
+           | [ H: ?R ?m, H': (forall R, R ?m -> _ ?m') |-
+               WeakestPrecondition.cmd ?_call ?_impl ?_tr ?m' ?_locals ?_post ] =>
+             apply H' in H; change (fun x => ?h x) with h in H
+           | [ m: mem, m': mem |- _ ] =>
+             match goal with
+             | [ H: forall R, R m -> _ m' |- _ ] => clear H
+             end
+           end.
+
+  Hint Extern 0 => simple eapply compile_alloc; cleanup_alloc; shelve.
+
+  Open Scope Z_scope.
+
+  (* FIXME (dustin): Replace Allocable with this? *)
+  Class Allocable {A} (P : word.rep -> A -> mem -> Prop) :=
+    { size_in_bytes : Z;
+      size_in_bytes_mod :
+        size_in_bytes mod Memory.bytes_per_word width = 0;
+      P_to_bytes px x :
+        Lift1Prop.impl1 (P px x) (Memory.anybytes px size_in_bytes);
+      P_from_bytes px :
+        Lift1Prop.impl1 (Memory.anybytes px size_in_bytes)
+                        (Lift1Prop.ex1 (P px)) }.
+
+  Instance Allocable_of_IAllocable {A} (P : word.rep -> A -> mem -> Prop)
+           {H: Allocable P} : Alloc.Allocable (fun _: unit => P).
+  Proof.
+    refine {| Alloc.size_in_bytes := size_in_bytes;
+              Alloc.size_in_bytes_mod := size_in_bytes_mod;
+              Alloc.P_to_bytes := _;
+              Alloc.P_from_bytes := _ |}; intros.
+    - apply P_to_bytes.
+    - abstract (red; exists tt; apply P_from_bytes; assumption).
+  Defined.
+
+  (* FIXME move *)
+  Lemma bytes_per_width_bytes_per_word : forall width,
+      width >= 0 ->
+      Z.of_nat (Memory.bytes_per (width := width) access_size.word) = Memory.bytes_per_word width.
+  Proof.
+    intros; unfold Memory.bytes_per, Memory.bytes_per_word.
+    rewrite Z2Nat.id; try apply Z.div_pos; lia.
+  Qed.
+
+  Lemma bytes_per_wordwidth_bytes_per_word :
+      Z.of_nat (Memory.bytes_per (width := width) access_size.word) = Memory.bytes_per_word width.
+  Proof.
+    apply bytes_per_width_bytes_per_word.
+    pose proof word.width_pos; lia.
+  Qed.
+
+  Lemma split_bytes_per_word:
+    forall x : word,
+      Z.of_nat
+        (Datatypes.length
+           (HList.tuple.to_list
+              (LittleEndian.split (Memory.bytes_per (width := width) access_size.word)
+                                  (word.unsigned x)))) = Memory.bytes_per_word width.
+  Proof.
+    intros x.
+    rewrite HList.tuple.length_to_list.
+    apply bytes_per_wordwidth_bytes_per_word.
+  Qed.
+
+  Lemma word_width_round :
+      width = 8 * ((width + 7) / 8).
+  Proof. destruct width_cases; subst; reflexivity. Qed.
+
+  Program Instance Allocable_scalar : Allocable scalar :=
+    {| size_in_bytes := Memory.bytes_per_word width;
+       size_in_bytes_mod := Z_mod_same_full _;
+       P_to_bytes := _;
+       P_from_bytes := _ |}.
+  Next Obligation.
+    intros m Hm.
+    evar (bs: list byte);
+      assert (array ptsto (word.of_Z 1) px bs m) by (subst bs; apply Hm).
+    subst bs; erewrite <- split_bytes_per_word.
+    eapply array_1_to_anybytes; eauto.
+  Qed.
+  Next Obligation.
+    intros m Hm.
+    eapply anybytes_to_array_1 in Hm; destruct Hm as (bs & Harray & Hlen).
+    eexists.
+    eapply scalar_of_bytes in Harray; try eassumption.
+    2: rewrite Hlen.
+    all: destruct width_cases; subst; reflexivity || lia.
+  Qed.
+
+  Program Instance Allocable_cell : Allocable cell_value :=
+    {| size_in_bytes := Memory.bytes_per_word width;
+       size_in_bytes_mod := Z_mod_same_full _;
+       P_to_bytes := _;
+       P_from_bytes := _ |}.
+  Next Obligation.
+    apply (P_to_bytes (Allocable := Allocable_scalar)).
+  Qed.
+  Next Obligation.
+    intros m H.
+    edestruct (P_from_bytes (Allocable := Allocable_scalar) _ _ H).
+    exists {| data := x |}. assumption.
+  Qed.
+
   Derive indirect_add_three'_body SuchThat
          (defn! "indirect_add_three'"("out", "a", "b", "c") { indirect_add_three'_body },
           implements indirect_add_three' using ["indirect_add"])
-         As indirect_add_three'_body_correct.
+    As indirect_add_three'_body_correct.
   Proof.
-    compile.
-  Qed. *)
+    compile_setup.
+    compile_step.
+    compile_step.
+    compile_step.
+    eapply compile_nlet_as_nlet_eq.
+    simple eapply compile_alloc; cleanup_alloc.
+    (* FIXME when no instance is defined the typeclass goal is shelved; why? *)
+    compile_step.
+    compile_step.
+    compile_step.
+    compile_step.
+    compile_step.
+    compile_step.
+    compile_step.
+    compile_step.
+    compile_step.
+    compile_step.
+    compile_step.
+    compile_step.
+    compile_step.
+    (* FIXME at this point we've lost too much info: we lost most clauses that
+       talked about `m'`.  The problem is that the compilation lemmas assume
+       there's a single relevant clause.  Is this worth a refactoring so that we
+       propagate info about all statements about a given memory? *)
+  Abort.
 End with_parameters.
